verification/PacketPile2.dfy
@@ -73,7 +73,7 @@ class PacketPile
         invariant 0 <= i <= count; 
         invariant next <= almostTrashIDs.Length;
         invariant forall j :: 0 <= j < next ==> almostTrashIDs[j] == 1; 
-        invariant next == Count(buf[..i], 1)
+        invariant next == Count(buf[..i], 1);
         invariant next + Count(buf[i..count], 1) == almostTrashIDs.Length;
         invariant multiset(almostTrashIDs[..next]) <= multiset(buf[..i]);
         {
